concurrency/common/sepcomp.v
@@ -1,11 +1,11 @@
-Require  VST.concurrency.common.core_semantics.
+(*Require  VST.concurrency.common.core_semantics.*)
 Require  VST.sepcomp.mem_lemmas.
 Require  VST.sepcomp.structured_injections.
 Require  VST.sepcomp.effect_semantics.
 Require  VST.sepcomp.extspec.
 Require  VST.sepcomp.Address.
 Module SepComp.
- Export VST.concurrency.common.core_semantics.
+(* Export VST.concurrency.common.core_semantics.*)
  Export VST.sepcomp.mem_lemmas.
  Export VST.sepcomp.structured_injections.
  Export VST.sepcomp.effect_semantics.
